src/high/resources/gen_ghost_map_map.v
@@ -38,7 +38,7 @@ Section definitions.
   Context `{!nvmBaseGS Σ Ω, !ghost_map_mapGpreS K1 K2 V Σ Ω, Inhabited V}.
   Implicit Types (m : gmap K1 (gmap K2 V)).
   Implicit Types (mi : gmap K2 V).
-  Implicit Types (dq: dfrac) (γ: gname) (bumper: V → option V).
+  Implicit Types (dq: dfrac) (γ: gname) (bumper: V → option V) (v: V).
 
   (* TODO: make these two assumption into a typeclass *)
   Context `{!ghost_mapGpreS loc (V → option V) Σ Ω}. (* ghost map for bumpers *)
@@ -50,22 +50,91 @@ Section definitions.
   (* Ownership over the entire map. *)
   Definition full_map γ dq m : iProp Σ :=
     ∃ (gnames : gmap loc gname),
-      ghost_map_auth γ loc_map_rel dq gnames ∗
+      ghost_map_auth γ drop_OCV dq gnames ∗
         ([∗ map] k1 ↦ γm;mi ∈ gnames;m,
-           ∃ bumper, k1 ↪[γbumper, loc_map_rel]□ bumper ∗
-                     ghost_map_auth γm (per_loc_map_rel k1 bumper) (dfrac_div_2 dq) mi).
+           ∃ bumper, k1 ↪[γbumper, drop_OCV]□ bumper ∗
+                     ghost_map_auth γm (drop_above_bump k1 bumper) (dfrac_div_2 dq) mi).
 
   (* Ownership over the entire history for a single key. *)
   Definition full_entry γ k1 dq mi : iProp Σ :=
-    ∃ γm bumper, k1 ↪[γ, loc_map_rel]□ γm ∗
-                 k1 ↪[γbumper, loc_map_rel]□ bumper ∗
-                 ghost_map_auth γm (per_loc_map_rel k1 bumper) (dfrac_div_2 dq) mi.
+    ∃ γm bumper, k1 ↪[γ, drop_OCV]□ γm ∗
+                 k1 ↪[γbumper, drop_OCV]□ bumper ∗
+                 ghost_map_auth γm (drop_above_bump k1 bumper) (dfrac_div_2 dq) mi.
 
   Definition frag_entry γ k1 k2 v : iProp Σ :=
-    ∃ γm bumper, k1 ↪[γ, loc_map_rel]□ γm ∗
-                    k1 ↪[γbumper, loc_map_rel]□ bumper ∗
-                    k2 ↪[γm, per_loc_map_rel k1 bumper]□ v.
+    ∃ γm bumper, k1 ↪[γ, drop_OCV]□ γm ∗
+                    k1 ↪[γbumper, drop_OCV]□ bumper ∗
+                    k2 ↪[γm, drop_above_bump k1 bumper]□ v.
+
+  (** The last generation map assertions *)
+  
+  (* Ownership over the entire map. *)
+  Definition lastgen_full_map γ dq m : iProp Σ :=
+    ∃ (gnames : gmap loc gname),
+      lastgen_ghost_map_auth γ dq gnames ∗
+        ([∗ map] k1 ↦ γm;mi ∈ gnames;m,
+           lastgen_ghost_map_auth γm (dfrac_div_2 dq) mi).
+
+  (* Ownership over the entire history for a single key. *)
+  Definition lastgen_full_entry γ k1 dq mi : iProp Σ :=
+    ∃ γm, lastgen_ghost_map_elem γ k1 DfracDiscarded γm ∗
+          lastgen_ghost_map_auth γm (dfrac_div_2 dq) mi.
+  
+  Definition lastgen_frag_entry γ k1 k2 v : iProp Σ :=
+    ∃ γm, lastgen_ghost_map_elem γ k1 DfracDiscarded γm ∗
+          lastgen_ghost_map_elem γm k2 DfracDiscarded v.
 End definitions.
+
+(** We do not need all the lemmas for lastgen assertions
+ ** We are mostly interested in lookup and persist lemmas. *)
+Section lastgen_lemmas.
+  Notation K1 := loc.
+  Notation K2 := nat.
+  Notation V := positive.
+  Context `{!nvmBaseGS Σ Ω, !ghost_map_mapGpreS K1 K2 V Σ Ω}.
+  Implicit Types (m : gmap K1 (gmap K2 V)).
+  Implicit Types (mi : gmap K2 V).
+  Implicit Types (dq: dfrac) (γ: gname) (bumper: V → option V).
+  Lemma lastgen_full_map_persist {γ} q m :
+    lastgen_full_map γ (DfracOwn q) m ==∗ lastgen_full_map γ DfracDiscarded m.
+  Proof.
+    iDestruct 1 as (?) "[auth map]".
+    iExists _.
+    iMod (lastgen_ghost_map_auth_persist with "auth") as "$".
+    iApply big_sepM2_bupd.
+    iApply (big_sepM2_impl with "map").
+    iIntros "!>" (?????) "authI".
+    iMod (lastgen_ghost_map_auth_persist with "authI") as "$".
+    done.
+  Qed.
+
+  Lemma lastgen_full_map_frag_entry γ k1 k2 dq1 m v :
+    lastgen_full_map γ dq1 m -∗
+    lastgen_frag_entry γ k1 k2 v -∗
+    ∃ mi, ⌜ m !! k1 = Some mi ⌝ ∗ ⌜ mi !! k2 = Some v ⌝.
+  Proof.
+    iDestruct 1 as (gnames) "(auth & map)".
+    iDestruct 1 as (γm) "[#ptsγp #ptsv]".
+    iDestruct (lastgen_ghost_map_lookup with "auth ptsγp") as %look.
+    iDestruct (big_sepM2_lookup_l with "map") as (mi mLook) "authI"; first done.
+    iExists mi.
+    iDestruct (lastgen_ghost_map_lookup with "authI ptsv") as %->.
+    done.
+  Qed.
+
+  Lemma lastgen_full_map_full_entry γ k1 dq1 dq2 m mi :
+    lastgen_full_map γ dq1 m -∗
+    lastgen_full_entry γ k1 dq2 mi -∗
+    ⌜ m !! k1 = Some mi ⌝.
+  Proof.
+    iDestruct 1 as (gnames) "(auth & map)".
+    iDestruct 1 as (γm) "[pts authI]".
+    iDestruct (lastgen_ghost_map_lookup with "auth pts") as %look.
+    iDestruct (big_sepM2_lookup_l with "map") as (mi' mLook) "authI'"; first done.
+    iDestruct (lastgen_ghost_map_auth_agree with "authI authI'") as %->.
+    done.
+  Qed.
+End lastgen_lemmas.
 
 Section lemmas.
   Notation K1 := loc.
@@ -157,17 +226,17 @@ Section lemmas.
   Local Lemma full_entry_alloc_big {OCV OPV} m :
     crashed_at_offset OCV -∗
     rely_self crashed_at_name (crashed_at_pred OPV) -∗
-    ([∗set] k1 ∈ dom m, ∃ bumper, k1 ↪[γbumper, loc_map_rel]□ bumper) ==∗
+    ([∗set] k1 ∈ dom m, ∃ bumper, k1 ↪[γbumper, drop_OCV]□ bumper) ==∗
     ∃ gnames,
       ([∗ map] k1 ↦ γm;mi ∈ gnames;m,
-         ∃ bumper, k1 ↪[γbumper, loc_map_rel]□ bumper ∗
-                   ghost_map_auth γm (per_loc_map_rel k1 bumper) (dfrac_div_2 (DfracOwn 1)) mi) ∗
+         ∃ bumper, k1 ↪[γbumper, drop_OCV]□ bumper ∗
+                   ghost_map_auth γm (drop_above_bump k1 bumper) (dfrac_div_2 (DfracOwn 1)) mi) ∗
       ([∗ map] k1 ↦ γm;mi ∈ gnames;m,
-         ∃ bumper, k1 ↪[γbumper, loc_map_rel]□ bumper ∗
-                   ghost_map_auth γm (per_loc_map_rel k1 bumper) (dfrac_div_2 (DfracOwn 1)) mi) ∗
+         ∃ bumper, k1 ↪[γbumper, drop_OCV]□ bumper ∗
+                   ghost_map_auth γm (drop_above_bump k1 bumper) (dfrac_div_2 (DfracOwn 1)) mi) ∗
       ([∗ map] k1 ↦ γm;mi ∈ gnames;m,
-         ∃ bumper, k1 ↪[γbumper, loc_map_rel]□ bumper ∗
-                   ([∗ map] k2 ↦ v ∈ mi, k2 ↪[γm, per_loc_map_rel k1 bumper]□ v)).
+         ∃ bumper, k1 ↪[γbumper, drop_OCV]□ bumper ∗
+                   ([∗ map] k2 ↦ v ∈ mi, k2 ↪[γm, drop_above_bump k1 bumper]□ v)).
   Proof.
     setoid_rewrite <- big_sepM2_sep. setoid_rewrite <- big_sepM2_sep.
     induction m as [|k1 mi m ? IH] using map_ind.
@@ -179,7 +248,7 @@ Section lemmas.
       iMod (IH with "crashed_at crashed_rely bumpers") as (gnames) "M".
       iDestruct (big_sepM2_dom with "M") as %domEq.
       iMod (ghost_map_alloc_persistent
-              OPV OCV (per_loc_map_rel k1 bumper) mi with "crashed_at crashed_rely") as (γ1) "[auth discard]".
+              (drop_above_bump k1 bumper) OPV OCV mi with "crashed_at crashed_rely") as (γ1) "[auth discard]".
       iExists (<[ k1 := γ1 ]> gnames).
       iModIntro.
       rewrite big_sepM2_insert; try done.
@@ -197,7 +266,7 @@ Section lemmas.
   Qed.
   
   Lemma full_map_alloc OPV OCV m :
-    ([∗set] k1 ∈ dom m, ∃ bumper, k1 ↪[γbumper, loc_map_rel]□ bumper) -∗
+    ([∗set] k1 ∈ dom m, ∃ bumper, k1 ↪[γbumper, drop_OCV]□ bumper) -∗
     crashed_at_offset OCV -∗
     rely_self crashed_at_name (crashed_at_pred OPV) ==∗
     ∃ γ, full_map γbumper γ (DfracOwn 1) m ∗
@@ -207,7 +276,7 @@ Section lemmas.
     rewrite /full_map /full_entry.
     iIntros "#bumpers #crashed_at_offset #rely_self".
     iMod (full_entry_alloc_big m with "[#$] [#$] bumpers") as (gnames) "(M1 & M2 & F)".
-    iMod (ghost_map_alloc_persistent OPV OCV loc_map_rel gnames with "[#$] [#$]") as (γ) "[H1 #ptsMap]".
+    iMod (ghost_map_alloc_persistent drop_OCV OPV OCV gnames with "[#$] [#$]") as (γ) "[H1 #ptsMap]".
     iExists γ.
     rewrite bi.sep_exist_r.
     iExists (gnames).
@@ -291,7 +360,7 @@ Section lemmas.
   Lemma full_map_insert γ m k1 bumper mi :
     m !! k1 = None →
     (∃ OPV, rely_self crashed_at_name (crashed_at_pred OPV)) -∗
-    k1 ↪[γbumper, loc_map_rel]□ bumper -∗
+    k1 ↪[γbumper, drop_OCV]□ bumper -∗
     full_map γbumper γ (DfracOwn 1) m ==∗
       full_map γbumper γ (DfracOwn 1) (<[k1 := mi]> m) ∗
       full_entry γbumper γ k1 (DfracOwn 1) mi ∗
@@ -304,13 +373,13 @@ Section lemmas.
     (* extract [crashed_at_offset] from existing resource *)
     iDestruct (ghost_map_auth_crashed_at_offset with "auth") as (OCV) "#crashed_at_offset".
     (* Allocate the ghost state for the entry. *)
-    iMod (ghost_map_alloc_persistent OPV OCV (per_loc_map_rel k1 bumper) mi with "[#$] [#$]") as (γm) "[authI pts2]".
+    iMod (ghost_map_alloc_persistent (drop_above_bump k1 bumper) OPV OCV mi with "[#$] [#$]") as (γm) "[authI pts2]".
     iEval (rewrite -Qp.half_half -dfrac_op_own ghost_map_auth_fractional) in "authI".
     replace (DfracOwn (1 / 2)) with (dfrac_div_2 (DfracOwn 1)); last done.
     iDestruct "authI" as "[authI authI']".
     assert (gnames !! k1 = None).
     { apply not_elem_of_dom. rewrite domEq. apply not_elem_of_dom. done. }
-    iMod (ghost_map_insert_persist k1 γm with "auth") as "[auth #pts]";
+    iMod (ghost_map_insert_persist _ k1 γm with "auth") as "[auth #pts]";
       first done.
     iModIntro. iSplitL "auth authI map".
     { iExists (<[k1 := _]> gnames).
@@ -343,7 +412,7 @@ Section lemmas.
     iDestruct (ghost_map_elem_agree with "bumper bumper'") as %<-.
     iCombine "authI authI'" as "authI".
     iEval (rewrite -ghost_map_auth_fractional Qp.half_half) in "authI".
-    iMod (ghost_map_insert_persist k2 v with "authI") as "[authI ptsI]";
+    iMod (ghost_map_insert_persist _ k2 v with "authI") as "[authI ptsI]";
       first done.
     iEval (rewrite -Qp.half_half -dfrac_op_own ghost_map_auth_fractional) in "authI".
     replace (DfracOwn (1 / 2)) with (dfrac_div_2 (DfracOwn 1)); last done.
@@ -365,7 +434,7 @@ Section lemmas.
     rewrite /full_entry /frag_entry.
     iDestruct 1 as (γm bumper) "(#topPts & #bumper & M)".
     iIntros "H". simpl.
-    iApply (ghost_map_lookup_big (dq := DfracDiscarded) with "M").
+    iApply (ghost_map_lookup_big with "M").
     iApply (big_sepM_impl with "H").
     iModIntro. iIntros (???).
     iIntros "(% & % & hi & bumper' & ho)".
@@ -440,11 +509,15 @@ Section Nextgen.
   
   (* Since we need to have some notion of global bumpers, it's difficult to make it
    * work with the [IntoNextgen] typeclass. *)
+  (* TODO: last gen *)
   Lemma full_map_nextgen dq1 dq2 abs_hists:
     full_map γbumper γ dq1 abs_hists -∗
-    ghost_map_auth γbumper loc_map_rel dq2 bumpers -∗
-    ghost_map_auth γbumper loc_map_rel dq2 bumpers ∗
-    ⚡==> ∀ OCV, crashed_at_offset OCV -∗ full_map γbumper γ dq1 (abs_hist_trans OCV abs_hists).
+    ghost_map_auth γbumper drop_OCV dq2 bumpers -∗
+    ghost_map_auth γbumper drop_OCV dq2 bumpers ∗
+    ⚡==>
+      lastgen_full_map γ dq1 abs_hists ∗
+      ∀ OCV, crashed_at_offset OCV -∗
+             full_map γbumper γ dq1 (abs_hist_trans OCV abs_hists).
   Proof.
     iIntros "(%gnames & gnames_auth & abs_hists_auth) bumpers".
     iDestruct (big_sepM2_dom with "abs_hists_auth") as %domEq.
@@ -461,11 +534,12 @@ Section Nextgen.
       by eexists. }
     iPoseProof (big_sepM2_impl_dom_subseteq_with_resource _
                   (λ ℓ gname abs_hist,
-                     ⚡==> ∃ bump, 
+                     ⚡==> lastgen_ghost_map_auth gname (dfrac_div_2 dq1) abs_hist ∗
+                         ∃ bump, 
                          ⌜ bumpers !! ℓ = Some bump ⌝ ∗
                          ∀ OCV, crashed_at_offset OCV -∗ ⌜ ℓ ∈ dom OCV ⌝ -∗
-                                ℓ ↪[γbumper,loc_map_rel]□ bump ∗
-                                ghost_map_auth gname (per_loc_map_rel ℓ bump) (dfrac_div_2 dq1) (drop_bump_map ℓ bump OCV abs_hist))%I
+                                ℓ ↪[γbumper,drop_OCV]□ bump ∗
+                                ghost_map_auth gname (drop_above_bump ℓ bump) (dfrac_div_2 dq1) (drop_bump_map ℓ bump OCV abs_hist))%I
                   gnames abs_hists gnames abs_hists with "bumpers abs_hists_auth []")
       as "[$ abs_hists_auth]"; [ done | done | | ].
     - iIntros "!>" (ℓ gname abs_hist gname' abs_hist' ????) "allBumpers entry".
@@ -474,14 +548,21 @@ Section Nextgen.
       iDestruct (ghost_map_lookup with "allBumpers knowBumper") as %bumperLook.
       iFrame "allBumpers".
       iModIntro.
+      iDestruct "fullEntry" as "[$ fullEntry]".
       iExists bump. iSplit; first done.
       iIntros (?) "#offset domOCV".
+      iDestruct "knowBumper" as "[_ knowBumper]".
       iSpecialize ("knowBumper" with "offset domOCV").
       iSpecialize ("fullEntry" with "offset").
       iFrame.
     - iDestruct (big_sepM2_alt with "abs_hists_auth") as (_) "abs_hists_auth".
       rewrite nextgen_big_sepM.
-      iIntros "!>" (OCV) "#offset".
+      iModIntro.
+      iDestruct "gnames_auth" as "[lastgen_gnames_auth gnames_auth]".
+      iDestruct (big_sepM_sep with "abs_hists_auth") as "[lastgen_abs_hists_auth abs_hists_auth]".
+      iSplitL "lastgen_gnames_auth lastgen_abs_hists_auth".
+      { iExists gnames. rewrite big_sepM2_alt. by iFrame. }
+      iIntros (OCV) "#offset".
       iSpecialize ("gnames_auth" with "offset").
       iExists (restrict (dom OCV) gnames).
       iFrame.
@@ -529,8 +610,8 @@ Section Nextgen.
 
   Lemma full_entry_nextgen ℓ dq1 dq2 abs_hist:
     full_entry γbumper γ ℓ dq1 abs_hist -∗
-    ghost_map_auth γbumper loc_map_rel dq2 bumpers -∗
-    ghost_map_auth γbumper loc_map_rel dq2 bumpers ∗
+    ghost_map_auth γbumper drop_OCV dq2 bumpers -∗
+    ghost_map_auth γbumper drop_OCV dq2 bumpers ∗
     ⚡==> ∀ OCV, crashed_at_offset OCV -∗ ⌜ ℓ ∈ dom OCV ⌝ -∗
                  match per_loc_trans OCV ℓ abs_hist with
                  | Some abs_hist' => full_entry γbumper γ ℓ dq1 abs_hist'
@@ -544,8 +625,11 @@ Section Nextgen.
     iFrame "allBumpers".
     iModIntro.
     iIntros (?) "#offset %domOCV".
+    iDestruct "knowGname" as "[_ knowGname]".
     iSpecialize ("knowGname" with "offset [//]").
+    iDestruct "knowBumper" as "[_ knowBumper]".
     iSpecialize ("knowBumper" with "offset [//]").
+    iDestruct "fullEntry" as "[_ fullEntry]".
     iSpecialize ("fullEntry" with "offset").
     rewrite /full_entry.
     iExists _, _. iFrame "∗#".
@@ -554,8 +638,8 @@ Section Nextgen.
   Lemma all_loc_full_entry_nextgen abs_hists dq1 dq2:
     dom abs_hists ⊆ dom bumpers →
     ([∗ map] ℓ ↦ abs_hist ∈ abs_hists, full_entry γbumper γ ℓ dq1 abs_hist) -∗
-    ghost_map_auth γbumper loc_map_rel dq2 bumpers -∗
-    ghost_map_auth γbumper loc_map_rel dq2 bumpers ∗
+    ghost_map_auth γbumper drop_OCV dq2 bumpers -∗
+    ghost_map_auth γbumper drop_OCV dq2 bumpers ∗
     ⚡==> ∀ OCV, crashed_at_offset OCV -∗
                  ([∗ map] ℓ ↦ abs_hist ∈ (abs_hist_trans OCV abs_hists), full_entry γbumper γ ℓ dq1 abs_hist).
   Proof.
@@ -591,9 +675,10 @@ Section Nextgen.
   Lemma frag_entry_nextgen ℓ t v bumper dq:
     bumpers !! ℓ = Some bumper →
     frag_entry γbumper γ ℓ t v -∗
-    ghost_map_auth γbumper loc_map_rel dq bumpers -∗
-    ghost_map_auth γbumper loc_map_rel dq bumpers ∗
-    ⚡==> ∀ OCV, crashed_at_offset OCV -∗ ⌜ ℓ ∈ dom OCV ⌝ -∗
+    ghost_map_auth γbumper drop_OCV dq bumpers -∗
+    ghost_map_auth γbumper drop_OCV dq bumpers ∗
+    ⚡==> lastgen_frag_entry γ ℓ t v ∗
+          ∀ OCV, crashed_at_offset OCV -∗ ⌜ ℓ ∈ dom OCV ⌝ -∗
                  match drop_above_bump ℓ bumper OCV t v with
                  | Some v' => frag_entry γbumper γ ℓ t v'
                  | None => emp
@@ -604,8 +689,13 @@ Section Nextgen.
     iFrame "allBumpers".
     simplify_map_eq.
     iModIntro.
+    iDestruct "knowGname" as "[l1 knowGname]".
+    iDestruct "entry" as "[l2 entry]".
+    iSplitL "l1 l2".
+    { iExists _. iFrame "∗#". }
     iIntros (?) "#offset %domOCV".
     iSpecialize ("knowGname" with "offset [//]").
+    iDestruct "knowBumper" as "[_ knowBumper]".
     iSpecialize ("knowBumper" with "offset [//]").
     iSpecialize ("entry" with "offset").
     destruct (drop_above_bump ℓ bumper OCV t v); last done.
@@ -615,9 +705,10 @@ Section Nextgen.
   Lemma per_loc_frag_entry_nextgen ℓ abs_hist bumper dq:
     bumpers !! ℓ = Some bumper →
     ([∗ map] t ↦ encσ ∈ abs_hist, frag_entry γbumper γ ℓ t encσ) -∗
-    ghost_map_auth γbumper loc_map_rel dq bumpers -∗
-    ghost_map_auth γbumper loc_map_rel dq bumpers ∗
-    ⚡==> ∀ OCV, crashed_at_offset OCV -∗ ⌜ ℓ ∈ dom OCV ⌝ -∗
+    ghost_map_auth γbumper drop_OCV dq bumpers -∗
+    ghost_map_auth γbumper drop_OCV dq bumpers ∗
+    ⚡==> ([∗ map] t ↦ encσ ∈ abs_hist, lastgen_frag_entry γ ℓ t encσ) ∗
+          ∀ OCV, crashed_at_offset OCV -∗ ⌜ ℓ ∈ dom OCV ⌝ -∗
                  match per_loc_trans OCV ℓ abs_hist with
                  | Some abs_hist' => ([∗ map] t ↦ encσ ∈ abs_hist', frag_entry γbumper γ ℓ t encσ)
                  | None => emp
@@ -633,6 +724,7 @@ Section Nextgen.
     - simpl.
       rewrite nextgen_big_sepM.
       iModIntro.
+      iDestruct (big_sepM_sep with "entries") as "[$ entries]".
       iIntros (?) "#offset %domOCV".
       rewrite /per_loc_trans bumperLook.
       iDestruct (big_sepM_impl_dom_subseteq _ _ _ (drop_bump_map ℓ bumper OCV abs_hist) with "entries []") as "[$ _]".
@@ -646,37 +738,16 @@ Section Nextgen.
       destruct (decide _); last done.
       by rewrite absHistLook'.
   Qed.
-
-  (* This version uses per-location bumper knowledge *)
-  Lemma frag_entry_local_nextgen ℓ t v bumper:
-    frag_entry γbumper γ ℓ t v -∗
-    ℓ ↪[γbumper, loc_map_rel]□ bumper -∗
-    ⚡==> ∀ OCV, crashed_at_offset OCV -∗ ⌜ ℓ ∈ dom OCV ⌝ -∗
-                 match drop_above_bump ℓ bumper OCV t v with
-                 | Some v' => frag_entry γbumper γ ℓ t v'
-                 | None => emp
-                 end.
-  Proof.
-    iIntros "(%γm & %bumper' & #knowGname & #knowBumper & entry) #knowBumper'".
-    iDestruct (ghost_map_elem_agree with "knowBumper knowBumper'") as %->.
-    iClear "knowBumper'".
-    simplify_map_eq.
-    iModIntro.
-    iIntros (?) "#offset %domOCV".
-    iSpecialize ("knowGname" with "offset [//]").
-    iSpecialize ("knowBumper" with "offset [//]").
-    iSpecialize ("entry" with "offset").
-    destruct (drop_above_bump ℓ bumper OCV t v); last done.
-    iExists _, _. iFrame "∗#".
-  Qed.
   
   Lemma all_loc_frag_entry_nextgen abs_hists dq:
     dom abs_hists = dom bumpers →
     ([∗ map] ℓ ↦ abs_hist ∈ abs_hists,
        [∗ map] t ↦ encσ ∈ abs_hist, frag_entry γbumper γ ℓ t encσ) -∗
-    ghost_map_auth γbumper loc_map_rel dq bumpers -∗
-    ghost_map_auth γbumper loc_map_rel dq bumpers ∗
-    ⚡==> ∀ OCV, crashed_at_offset OCV -∗
+    ghost_map_auth γbumper drop_OCV dq bumpers -∗
+    ghost_map_auth γbumper drop_OCV dq bumpers ∗
+    ⚡==> ([∗ map] ℓ ↦ abs_hist ∈ abs_hists,
+             [∗ map] t ↦ encσ ∈ abs_hist, lastgen_frag_entry γ ℓ t encσ) ∗
+          ∀ OCV, crashed_at_offset OCV -∗
                  ([∗ map] ℓ ↦ abs_hist ∈ abs_hist_trans OCV abs_hists,
                     [∗ map] t ↦ encσ ∈ abs_hist, frag_entry γbumper γ ℓ t encσ).
   Proof.
@@ -692,6 +763,7 @@ Section Nextgen.
     - simpl.
       rewrite nextgen_big_sepM.
       iModIntro.
+      iDestruct (big_sepM_sep with "all_entries") as "[$ all_entries]".
       iIntros (?) "#offset".
       iDestruct (big_sepM_impl_dom_subseteq _ _ _ (abs_hist_trans OCV abs_hists) with "all_entries []") as "[$ _]".
       { rewrite /abs_hist_trans restrict_dom_L.
@@ -704,6 +776,49 @@ Section Nextgen.
       iSpecialize ("entries" with "offset [//]").
       rewrite /abs_hist_trans restrict_lookup_elem_of // map_lookup_imap absHistsLook /= in absHistsLook'.
       by rewrite absHistsLook'.
+  Qed.
+  
+  (* This version uses per-location bumper knowledge *)
+  Lemma frag_entry_local_nextgen ℓ t v:
+    frag_entry γbumper γ ℓ t v -∗
+    ⚡==>
+      lastgen_frag_entry γ ℓ t v ∗
+      ∀ OCV bumper, crashed_at_offset OCV -∗ ⌜ ℓ ∈ dom OCV ⌝ -∗
+           ℓ ↪[γbumper, drop_OCV]□ bumper -∗
+           match drop_above_bump ℓ bumper OCV t v with
+           | Some v' => frag_entry γbumper γ ℓ t v'
+           | None => emp
+           end.
+  Proof.
+    iIntros "(%γm & %bumper' & #knowGname & #knowBumper & entry)".
+    iModIntro.
+    iDestruct "knowGname" as "[l1 knowGname]".
+    iDestruct "entry" as "[l2 entry]".
+    iSplitL "l1 l2".
+    { iExists _. by iFrame. }
+    iIntros (??) "#offset %domOCV knowBumper'".
+    iDestruct "knowBumper" as "[_ knowBumper]".
+    iSpecialize ("knowBumper" with "offset [//]").
+    iDestruct (ghost_map_elem_agree with "knowBumper knowBumper'") as %->.
+    iSpecialize ("knowGname" with "offset [//]").
+    iSpecialize ("entry" with "offset").
+    destruct (drop_above_bump ℓ bumper OCV t v); last done.
+    iExists _, _. iFrame "∗#".
+  Qed.
+
+  #[global] Instance frag_entry_local_into_nextgen ℓ t v:
+    IntoNextgen
+      (frag_entry γbumper γ ℓ t v)
+      (lastgen_frag_entry γ ℓ t v ∗
+       ∀ OCV bumper, crashed_at_offset OCV -∗ ⌜ ℓ ∈ dom OCV ⌝ -∗
+           ℓ ↪[γbumper, drop_OCV]□ bumper -∗
+           match drop_above_bump ℓ bumper OCV t v with
+           | Some v' => frag_entry γbumper γ ℓ t v'
+           | None => emp
+           end).
+  Proof.
+    rewrite /IntoNextgen.
+    iApply frag_entry_local_nextgen.
   Qed.
 End Nextgen.
 
