src/high/recovery_weakestpre.v
@@ -12,7 +12,7 @@ From self.high Require Import dprop generational_resources wrappers protocol.
 From self Require Import view map_extra extra ipm_tactics if_non_zero view_slice solve_view_le.
 From self.base Require Import primitive_laws wpr_lifting.
 From self.high Require Import generational_resources crash_weakestpre.
-From self.high.modalities Require Import or_lost nextgen.
+From self.high.modalities Require Import nextgen.
 From self.nextgen Require Import nextgen_promises.
 
 Set Default Proof Using "Type*".
@@ -111,34 +111,44 @@ Section wpr.
     intros ℓ look.
     apply elem_of_dom in look as [].
     eapply (map_Forall_lookup_1 _ _ _ _ H'); done.
-  Qed.
+  Qed.  
   Opaque nvm_heap_ctx.
-  
+
   Lemma extra_state_nextgen CV σ1 σ2:
     CV_crash_step CV σ1 σ2 →
-    crashed_at_offset OCV -∗
-    nvm_heap_ctx σ1 →
-    picked_out crashed_at_name (crashed_at_trans (OCV `view_add` CV)) -∗
+    nvm_heap_ctx σ1 -∗
     extra_state_interp -∗
-    |==> ▷ ⚡==> |==> extra_state_interp ∗ (∃ OCV, crashed_at_offset OCV ∗ crashed_in_impl OCV).
+    |==> ▷ ⚡==> |==> frag_history_at_crash ∗ nvm_heap_ctx σ2 ∗ extra_state_interp.
   Proof.
     intros Hcrash.
-    iIntros "#crashed_at_offset heap #mainpicked".
+    iIntros "heap".
     iNamed 1.
     (* basic pure information *)
     iDestruct (big_sepM2_dom with "bumperSome") as %domAbsHistsBumpers.
     iDestruct (big_sepM2_dom with "predsFullReadHold") as %domPhysHistsAbsHists.
     iDestruct (big_sepM2_dom with "ordered") as %domAbsHistsOrders.
+    iDestruct (big_sepM2_dom with "oldViewsDiscarded") as %offsetsDom.
+    iAssert (∃ OCV, crashed_at_offset OCV)%I with "[offsets]" as (OCV) "#crashed_at_offset".
+    { iNamed "offsets".
+      by iExists _. }
     iAssert ⌜ ∀ ℓ : loc, ℓ ∈ dom offsets → offsets !! ℓ = Some (OCV !!0 ℓ) ⌝%I with "[offsets]" as %HOffsetOCV.
     { iNamed "offsets".
       iDestruct (crashed_at_offset_agree with "crashed_at_offset crashed") as %->.
+      done. }
+    (* we know that individual [phys_hist] and [abs_hist] has the same domain. *)
+    iAssert ⌜ map_Forall (λ _ '(phys_hist, abs_hist), dom phys_hist = dom abs_hist) (map_zip phys_hists abs_hists) ⌝%I as %domAbsHistPhysHist.
+    { iDestruct (big_sepM2_alt with "predsFullReadHold") as "[_ ?]".
+      iApply big_sepM_pure_1.
+      iApply (big_sepM_impl with "[$]").
+      iIntros "!>" (ℓ [phys_hist abs_hist] [? ?]%map_lookup_zip_Some).
+      iIntros "(% & % & % & % & % & % & ?)".
+      simpl in *.
+      iDestruct (big_sepM2_dom with "[$]") as %?.
       done. }
     (* information that requires the base interp to extract. *)
     iDestruct (nvm_heap_ctx_OCV_dom with "crashed_at_offset heap") as %[domOCVPV domOCVStore].
     iDestruct (nvm_heap_ctx_mapsto with "crashed_at_offset heap ptsMap") as %[domCVPhysHists physHistsEq].
     simpl in domCVPhysHists.
-
-    iPoseProof (offset_auth_picked_out with "mainpicked offsets") as "offsets".
 
     (* some resources require manually [nextgen] proof *)
     iDestruct (full_map_nextgen with "history allBumpers") as "[allBumpers history]".
@@ -148,7 +158,7 @@ Section wpr.
 
     set OCV' := (OCV `view_add` CV).
     set offsets' := (max_nat_car <$> restrict (dom offsets) OCV').
-
+    
     assert (dom (drop_above_map OCV' phys_hists) = dom (abs_hist_trans bumpers OCV' abs_hists)).
     { rewrite dom_abs_hist_trans; last set_solver.
       rewrite /drop_above_map.
@@ -169,46 +179,115 @@ Section wpr.
         apply elem_of_dom.
         destruct (OCV' !! ℓ); first done.
         simpl in look'. destruct look'. congruence. }
+
+    (* relation between persisted view and crash view. *)
+    iAssert ⌜ ∀ ℓ offset, offsets !! ℓ = Some offset → offset + (global_pview !!0 ℓ) ≤ OCV' !!0 ℓ ⌝%I as %pViewLb.
+    { iIntros (ℓ offset ?).
+      assert (ℓ ∈ dom offsets) by by apply elem_of_dom.
+      assert (ℓ ∈ dom phys_hists) as [phys_hist ?]%elem_of_dom by set_solver.
+      assert (ℓ ∈ dom abs_hists) as [abs_hist ?]%elem_of_dom by set_solver.
+      iDestruct (big_sepM2_lookup _ _ _ ℓ with "predsPersHold") as "predP".
+      { done. } { done. }
+      iDestruct "predP" as (encp_pers t_p offset' encσ_p msg_p predPersLook offsetLook' encσPLook msgPLook <-) "[persisted predP]".
+      assert (offset' = offset) as -> by by simplify_map_eq.
+      subst OCV'.
+      rewrite view_add_lookup_zero.
+      specialize (HOffsetOCV ℓ ltac:(done)).
+      simplify_map_eq.
+      rewrite /lookup_zero.
+      destruct (global_pview !! ℓ) as [[pview] | ]; simpl; last (iPureIntro; lia).
+      Transparent nvm_heap_ctx.
+      iNamed "heap".
+      destruct Hcrash as [store PV pIncl cut]. simpl in *.
+      iAssert ⌜ OCV0 = OCV ⌝%I as %->.
+      { iDestruct (crashed_at_offset_agree with "[crashed] crashed_at_offset") as %<-; last done.
+        by iExists _. }
+      iDestruct (persisted_auth_included with "crashed_at_offset pers persisted") as %incl.
+      iPureIntro.
+      assert ({[ℓ := MaxNat pview]} ⊑ OCV `view_add` CV `view_sub` OCV) as incl'.
+      { etrans; first apply incl.
+        apply view_sub_mono.
+        apply view_add_mono; done. }
+      rewrite view_included in incl'.
+      specialize (incl' ℓ).
+      rewrite lookup_singleton in incl'.
+      rewrite /view_add /view_sub map_lookup_imap /= lookup_merge /lookup_zero in incl'.
+      move: incl'.
+      destruct (OCV !! ℓ) as [[] | ] eqn:Heq1;
+        destruct (CV !! ℓ) as [[] | ] eqn:Heq2;
+        rewrite ?Heq1 ?Heq2 /=.
+      - intros incl'%Some_MaxNat_included.
+        lia.
+      - intros incl'%Some_MaxNat_included.
+        lia.
+      - intros incl'%Some_MaxNat_included.
+        lia.
+      - intros incl'. apply option_not_included_None in incl'. done. }
     
-    iAssert (nvm_heap_ctx σ1 ∗
-             |==> ⚡==> ([∗ map] ℓ ↦ phys_hist;abs_hist ∈ drop_above_map OCV' phys_hists;abs_hist_trans bumpers OCV' abs_hists,
-                      encoded_full_read_predicates_hold ℓ abs_hist phys_hist (const ∅ <$> restrict (dom OCV') na_views) offsets'
-                        (restrict (dom OCV') predicates_full) (restrict (dom OCV') predicates_read) ∗
-                      encoded_pers_predicate_holds ℓ abs_hist phys_hist ∅ offsets'
-                        (restrict (dom OCV') predicates_pers)))%I with "[heap predsFullReadHold predsPersHold]" as "predsHold".
-    { rewrite -nextgen_big_sepM2 -big_sepM2_bupd.
+    (* obtain the assertions after crash. *)    
+    iAssert (|==> ⚡==>
+             (crashed_at CV ∗ persisted (view_to_zero OCV') ∗ frag_history_at_crash) -∗
+             ([∗ map] ℓ ↦ phys_hist;abs_hist ∈ drop_above_map OCV' phys_hists;abs_hist_trans bumpers OCV' abs_hists,
+                encoded_full_read_predicates_hold ℓ abs_hist phys_hist (map_imap (drop_OCV_clear OCV') na_views) offsets'
+                  (restrict (dom OCV') predicates_full) (restrict (dom OCV') predicates_read) ∗
+                encoded_pers_predicate_holds ℓ abs_hist phys_hist (restrict (dom OCV') $ view_to_zero global_pview) offsets'
+                  (restrict (dom OCV') predicates_pers)))%I with "[predsFullReadHold predsPersHold]" as ">predsHold".
+    { (* TODO: make the lemma behave better *)
+      rewrite -bupd_mono; last rewrite -nextgen_mono; last iApply big_sepM2_impl_persist; last done.
+      rewrite -nextgen_big_sepM2 -big_sepM2_bupd.
       iPoseProof (big_sepM2_sep with "[$predsFullReadHold $predsPersHold]") as "predsHold".
-      iDestruct (big_sepM2_impl_dom_subseteq_with_resource _ _
-                _ _ (drop_above_map OCV' phys_hists) (abs_hist_trans bumpers OCV' abs_hists)
-                with "heap predsHold []") as "[$ $]".
+      iDestruct (big_sepM2_impl_dom_subseteq _ _
+                   _ _ (drop_above_map OCV' phys_hists) (abs_hist_trans bumpers OCV' abs_hists)
+                   with "predsHold []") as "$".
       { rewrite /drop_above_map.
         etrans; first apply dom_imap_subseteq.
         done. }
       { done. }
       iIntros "!>" (ℓ phys_hist abs_hist phys_hist' abs_hist' physHistsLook absHistsLook physHistsLook' absHistsLook')
-        "heap [predFR predP]".
-      assert (is_Some (bumpers !! ℓ)) as [bumper bumpersLook].
-      { rewrite -elem_of_dom -domAbsHistsBumpers elem_of_dom. by eexists. }
-      assert (is_Some (orders !! ℓ)) as [order ordersLook].
-      { rewrite -elem_of_dom -domAbsHistsOrders elem_of_dom. by eexists. }
+        "[predFR predP]".
+      (* some pure facts *)
+      assert (ℓ ∈ dom abs_hists) by (apply elem_of_dom; by eexists).
+      assert (ℓ ∈ dom bumpers) as [bumper bumpersLook]%elem_of_dom by set_solver.
+      assert (ℓ ∈ dom orders) as [order ordersLook]%elem_of_dom by set_solver.
       (* we only care about locations that survives *)
-      destruct (decide (ℓ ∈ dom OCV')) as [ elemOfOCV | ];
+      destruct (decide (ℓ ∈ dom OCV')) as [ elemOfOCV' | ];
         last (rewrite restrict_lookup_not_elem_of // in absHistsLook').
       assert (drop_bump_map ℓ bumper OCV' abs_hist = abs_hist') as <-.
       { rewrite /abs_hist_trans in absHistsLook'.
         rewrite restrict_lookup_elem_of // map_lookup_imap absHistsLook /= /per_loc_trans bumpersLook in absHistsLook'.
         by simplify_eq. }
-      pose proof elemOfOCV as [[t_c] OCVLook' ]%elem_of_dom.
+      pose proof elemOfOCV' as [[t_c] OCVLook' ]%elem_of_dom.
       assert (discard_msg_views <$> drop_above t_c phys_hist = phys_hist') as <-.
       { rewrite /drop_above_map map_lookup_imap physHistsLook /= in physHistsLook'.
         rewrite /drop_above_hist in physHistsLook'.
         rewrite OCVLook' /= in physHistsLook'.
         by simplify_eq. }
+      assert (dom (discard_msg_views <$> drop_above t_c phys_hist) = dom (drop_bump_map ℓ bumper OCV' abs_hist)).
+      { rewrite dom_fmap_L /drop_above /drop_bump_map /drop_above_map /drop_above_bump.
+        rewrite set_eq.
+        intros t.
+        rewrite ?elem_of_dom.
+        rewrite map_filter_lookup map_lookup_imap.
+        apply (map_Forall_lookup_1 _ _ ℓ (phys_hist, abs_hist)) in domAbsHistPhysHist;
+          last rewrite map_lookup_zip_Some //.
+        simpl in domAbsHistPhysHist.
+        destruct (abs_hist !! t) eqn:Hlook.
+        - assert (is_Some (phys_hist !! t)) as [? ->] by (rewrite -elem_of_dom domAbsHistPhysHist elem_of_dom //).
+          simpl.
+          rewrite /lookup_zero OCVLook' /=.
+          destruct (decide (t ≤ t_c)).
+          + rewrite option_guard_True //.
+          + rewrite option_guard_False //.
+            split; by intros ?%is_Some_None.
+        - assert (phys_hist !! t = None) as -> by (rewrite -not_elem_of_dom domAbsHistPhysHist not_elem_of_dom //).
+          simpl.
+          split; by intros ?%is_Some_None. }
+      
       iDestruct "predFR" as (encp_full encp_read offset predFullLook predReadLook offsetLook) "predFR".
       iEval (rewrite /encoded_pers_predicate_holds) in "predP".
       iDestruct "predP" as (encp_pers t_p offset' encσ_p msg_p predPersLook offsetLook' encσPLook msgPLook <-) "[persisted predP]".
       assert (offset' = offset) as -> by by simplify_map_eq.
-      assert ((OCV `view_add` CV) !!0 ℓ = t_c) as OCVLook0'.
+      assert (OCV' !!0 ℓ = t_c) as OCVLook0'.
       { rewrite /lookup_zero OCVLook' //. }
       assert (offset ≤ t_c).
       { subst OCV'.
@@ -233,44 +312,13 @@ Section wpr.
           apply Hsubset'; first done.
           rewrite elem_of_dom. by eexists.
         + destruct (CV !! ℓ); done. }
-      iAssert ⌜ offset + (global_pview !!0 ℓ) ≤ t_c ⌝%I as %pViewLb.
-      { rewrite /lookup_zero.
-        destruct (global_pview !! ℓ) as [[pview] | ]; simpl; last (iPureIntro; lia).
-        Transparent nvm_heap_ctx.
-        iNamed "heap".
-        destruct Hcrash as [store PV pIncl cut]. simpl in *.
-        iAssert ⌜ OCV0 = OCV ⌝%I as %->.
-        { iDestruct (crashed_at_offset_agree with "[crashed] crashed_at_offset") as %<-; last done.
-          by iExists _. }
-        iDestruct (persisted_auth_included with "crashed_at_offset pers persisted") as %incl.
-        iPureIntro.
-        assert ({[ℓ := MaxNat pview]} ⊑ OCV `view_add` CV `view_sub` OCV) as incl'.
-        { etrans; first apply incl.
-          apply view_sub_mono.
-          apply view_add_mono; done. }
-        rewrite view_included in incl'.
-        specialize (incl' ℓ).
-        rewrite lookup_singleton in incl'.
-        rewrite /view_add /view_sub map_lookup_imap /= lookup_merge /lookup_zero in incl'.
-        move: incl'.
-        rewrite tCLook'.
-        destruct (OCV !! ℓ) as [[] | ] eqn:Heq; rewrite ?Heq /=.
-        - intros incl'%Some_MaxNat_included.
-          simplify_map_eq.
-          rewrite view_add_lookup_zero /lookup_zero tCLook' Heq /=.
-          lia.
-        - intros incl'%Some_MaxNat_included.
-          simplify_map_eq.
-          rewrite view_add_lookup_zero /lookup_zero tCLook' Heq /=.
-          lia. }
-      iFrame "heap".
+      specialize (pViewLb ℓ offset ltac:(done)).
       iClear "persisted".
       
       destruct Hcrash as [store PV pIncl cut]. simpl in *.
       (* we should be able to find a message exactly at [t_c]. *)
       assert (is_Some (phys_hist !! t_c)) as [msg_c msgCLook].
-      { simpl in physHistsEq.
-        apply consistent_cut_valid_slice in cut as valid.
+      { apply consistent_cut_valid_slice in cut as valid.
         apply (valid_slice_lookup _ ℓ t_c' _ (drop_prefix phys_hist (OCV !!0 ℓ))) in valid; [ | done | ].
         - rewrite drop_prefix_lookup in valid.
           replace t_c with (t_c' + (OCV !!0 ℓ)); first done.
@@ -278,12 +326,16 @@ Section wpr.
           lia.
         - symmetry.
           eapply (map_Forall_lookup_1 _ _ _ _ physHistsEq); done. }
+      
       (* we can also derive that an (encoded) abstract state also exist at the timestamp. *)
       iDestruct (big_sepM2_dom with "predFR") as %domPhysHistAbsHist.
       assert (is_Some (abs_hist !! t_c)) as [encσ_c encσCLook].
       { rewrite -elem_of_dom -domPhysHistAbsHist elem_of_dom. by eexists. }
-      iPoseProof (big_sepM2_delete _ _ _ t_c msg_c encσ_c with "predFR") as "[predF predFRRest]".
+
+      (* we extract the predicate held at crash timestamp. *)
+      iPoseProof (big_sepM2_delete _ _ _ t_c msg_c encσ_c with "predFR") as "[predFR predFRRest]".
       { done. } { done. }
+      
       (* we know that [encσ_p ⊑ encσ_c] always holds. *)
       iAssert ⌜ order encσ_p encσ_c ∨ encσ_p = encσ_c ⌝%I as %orderPC.
       { destruct (decide (offset + (global_pview !!0 ℓ) = t_c)) as [ <- | ].
@@ -295,39 +347,59 @@ Section wpr.
           iPureIntro.
           eapply (incrMap _); try done.
           lia. }
+
       (* we know that bumper always return [Some _] *)
       iAssert ⌜ ∃ encσ_c', bumper encσ_c = Some encσ_c' ⌝%I as %[encσ_c' bumperSome].
       { iDestruct (big_sepM2_lookup _ _ _ ℓ with "bumperSome") as %bumperSome.
         { done. } { done. }
         iPureIntro.
         eapply (map_Forall_lookup_1 _ _ _ _ bumperSome); done. }
+
+      (* specialize the implication as much as possible *)
+      iDestruct (big_sepM2_lookup _ _ _ ℓ with "predFullNextgen") as (encp_full' encp_read' encp_pers' ? ? ?) "nextgen".
+      { done. }
+      { done. }
       destruct (phys_hist !! S t_c) as [msgSC | ] eqn:msgSCLook.
       - (* the crash timestamp is not exclusive, we need to apply the second case of [predFullNextgen] *)
         admit.
       - (* the crash timestamp is exclusive, we can apply the first case of [predFullNextgen]. *)
         rewrite decide_True; last done.
-        iDestruct (big_sepM2_lookup _ _ _ ℓ with "predFullNextgen") as (encp_full' encp_read' encp_pers' ? ? ?) "nextgen".
-        { done. }
-        { done. }
         clear OCVLook0'.
         simplify_map_eq.
         iDestruct (plainly_elim with "nextgen") as "NG".
-        iDestruct ("NG" with "[//] predP predF") as "[fullNG _]".
+        iDestruct ("NG" with "[//] predP predFR") as "[fullNG _]".
         iDestruct ("fullNG" with "[//]") as ">(%P_full' & %P_pers' & #PFullEquiv' & #PPersEquiv' & fullNG)".
-        (* For the rest of the predicates, we split them into two facts: *)
-    (*      * the persistent knowledge about predicate equivalence, *)
-    (*      * and the resource under [⚡==>] modality. *)
-        iPoseProof (big_sepM2_impl
-                     _
-                     (λ t msg_r encσ_r,
-                        (⚡==> ∀ (P: dProp Σ) encσ_r',
-                           ⌜ bumper encσ_r = Some encσ_r' ⌝ -∗
-                           encp_read encσ_r' msg_r.(msg_val) ≡ Some P -∗
-                           (⎡ persisted (view_to_zero (msg_persisted_after_view (msg_r))) ⎤ ∗ ⎡ crashed_at CV ⎤ -∗
-                            P) (∅, ∅, ∅))
-                        )%I
+        
+        iDestruct (big_sepM2_impl_dom_subseteq _
+                     (λ t msg_r encσ_r, ⚡==> (persisted (view_to_zero OCV') ∗ crashed_at CV ∗ frag_history_at_crash) -∗
+                                        encoded_predicate_holds encp_read encσ_r
+                                          (msg_val msg_r)
+                                          (∅, ∅, ∅))%I
+                     _ _ (delete t_c $ discard_msg_views <$> drop_above t_c phys_hist) (delete t_c $ drop_bump_map ℓ bumper OCV' abs_hist)
                      with "predFRRest []") as "predFRRest".
-        { iIntros "!>" (t msg_r encσ_r [? msgRLook]%lookup_delete_Some [_ encσRLook]%lookup_delete_Some) "predR".
+        { rewrite ?dom_delete dom_fmap /drop_above.
+          apply difference_mono_r, dom_filter_subseteq. }
+        { rewrite !dom_delete_L.
+          by f_equiv. }
+        { iIntros "!>" (t msg_r encσ_r msg_r' encσ_r' [? msgRLook]%lookup_delete_Some [_ encσRLook]%lookup_delete_Some [? msgRLook']%lookup_delete_Some [_ encσRLook']%lookup_delete_Some) "predR".
+          assert (msg_r' = discard_msg_views msg_r) as ->.
+          { apply lookup_fmap_Some in msgRLook' as (? & <- & msgRLook').
+            f_equiv.
+            apply map_filter_lookup_Some_1_1 in msgRLook'.
+            by simplify_map_eq. }
+          assert (t ≤ t_c).
+          { apply lookup_fmap_Some in msgRLook' as (? & _ & msgRLook').
+            by apply map_filter_lookup_Some_1_2 in msgRLook'. }
+          iAssert ⌜ Some encσ_r' = bumper encσ_r ⌝%I as %bumperSomeR.
+          { rewrite map_lookup_imap encσRLook /= /drop_above_bump in encσRLook'.
+            destruct (decide _); last done.
+            rewrite /safe_bumper in encσRLook'.
+            iDestruct (big_sepM2_lookup _ _ _ ℓ with "bumperSome") as %bumperSomeR.
+            { done. } { done. }
+            iPureIntro.
+            move: encσRLook'.
+            eapply map_Forall_lookup_1 in bumperSomeR as [? -> ]; last done.
+            done. }
           iAssert (encoded_predicate_holds encp_read encσ_r (msg_val msg_r)
                      (default (msg_store_view msg_r) (na_views !! ℓ), msg_persisted_after_view msg_r, ∅))%I with "[predR]" as "predR".
           { destruct (decide _); last done.
@@ -336,104 +408,377 @@ Section wpr.
             iDestruct ("split" with "predR") as "$". }
           iDestruct (big_sepM2_lookup _ _ _ ℓ with "predReadNextgen") as "nextgen'".
           { done. } { done. }
-          iAssert ⌜ ∃ encσ_r', bumper encσ_r = Some encσ_r' ⌝%I as %[encσ_r' bumperSomeR].
-          { iDestruct (big_sepM2_lookup _ _ _ ℓ with "bumperSome") as %bumperSomeR.
-            { done. } { done. }
-            iPureIntro.
-            eapply (map_Forall_lookup_1 _ _ _ _ bumperSomeR); done. }
           iDestruct ("nextgen'" $! encσ_r encσ_r' with "[//] predR") as (P) "[#encpReadEquiv' ReadNG]".
           iModIntro.
+          iIntros "#(persisted & CV & frag_impl)".
+          iSpecialize ("ReadNG" with "frag_impl").
+          iDestruct (big_sepM2_lookup _ _ _ ℓ with "oldViewsDiscarded") as %discarded.
+          { done. } { done. }
           iSpecialize ("ReadNG" $! CV with "[]").
-          { iSplitPure; first admit.
-            iSplit; first admit. (* FIXME: this one seems problematic. *)
-            admit. }
-          -
-          iApply "ReadNG".
-        }
-    }
+          (* [<NGF>] header *)
+          { simpl.
+            iFrame "CV".
+            assert (msg_persisted_after_view msg_r ⊑ CV).
+            { (* we need a different proof for messages from older generation. *)
+              destruct (decide (t < OCV !!0 ℓ)).
+              - rewrite -(discarded t _ ltac:(done) ltac:(done)) /=.
+                solve_view_le.
+              - eapply consistent_cut_extract.
+                +  done.
+                + done.
+                + apply (map_Forall_lookup_1 _ phys_hists ℓ phys_hist) in physHistsEq; last done.
+                  rewrite -physHistsEq //.
+                + rewrite drop_prefix_lookup.
+                  erewrite Nat.sub_add; first done.
+                  lia.
+                + rewrite PeanoNat.Nat.le_sub_le_add_l.
+                  subst OCV'.
+                  replace t_c' with (CV !!0 ℓ) by (rewrite /lookup_zero tCLook' //).
+                  rewrite -view_add_lookup_zero /lookup_zero OCVLook' /=.
+                  done. }
+            iSplitPure; first done.
+            iApply persisted_weak; last done.
+            f_equiv.
+            rewrite /OCV'.
+            replace (msg_persisted_after_view msg_r) with (∅ `view_add` msg_persisted_after_view msg_r)
+                                                          by apply view_add_empty.
+            f_equiv; solve_view_le. }
+          iExists P.
+          iFrame "∗#".}
+        rewrite nextgen_big_sepM2.
+        iIntros "!>!> #(CV & persisted & frag_impl)".
 
-    
-    (* we now pick the [crashed_at] resource using base logic nextgen lemma. *)
-    iDestruct (heap_ctx_next_generation _ _ _ Hcrash with "heap")
-      as ">[(%OCV' & #crashed_at_offset' & #picked_out) heap]".
-    iDestruct (crashed_at_offset_agree with "crashed_at_offset crashed_at_offset'") as %<-.
-    iClear "crashed_at_offset'".
-    destruct Hcrash as [store PV pIncl cut]. simpl in *.
-    
-    subst OCV'.
-    iModIntro. iModIntro.
+        (* restore [p_full] and [p_pers] *)
+        iSpecialize ("fullNG" with "frag_impl").
+        iDestruct ("fullNG" $! CV with "[]") as "[F P]".
+        (* [<NGF>] header *)
+        { simpl.
+          iFrame "CV".
+          assert (msg_persisted_after_view msg_c ⊑ CV).
+          { eapply consistent_cut_extract.
+            +  done.
+            + done.
+            + apply (map_Forall_lookup_1 _ phys_hists ℓ phys_hist) in physHistsEq; last done.
+              rewrite -physHistsEq //.
+            + rewrite drop_prefix_lookup.
+              erewrite Nat.sub_add; first done.
+              lia.
+            + rewrite PeanoNat.Nat.le_sub_le_add_l.
+              subst OCV'.
+              replace t_c' with (CV !!0 ℓ) by (rewrite /lookup_zero tCLook' //).
+              rewrite -view_add_lookup_zero /lookup_zero OCVLook' /=.
+              done. }
+          iSplitPure; first done.
+          iApply persisted_weak; last done.
+          f_equiv.
+          rewrite /OCV'.
+          replace (msg_persisted_after_view msg_c) with (∅ `view_add` msg_persisted_after_view msg_c)
+                                                        by apply view_add_empty.
+          f_equiv; solve_view_le. }
+        iSplitL "F predFRRest".
+        + iExists encp_full, encp_read, t_c.
+          iSplitPure; first rewrite restrict_lookup_elem_of //.
+          iSplitPure; first rewrite restrict_lookup_elem_of //.
+          iSplitPure.
+          { subst offsets'.
+            rewrite lookup_fmap restrict_lookup_elem_of; first rewrite OCVLook' //.
+            rewrite elem_of_dom //. }
+          iApply (big_sepM2_delete _ _ _ t_c with "[F predFRRest]").
+          { rewrite lookup_fmap (map_filter_lookup_Some_2 _ _ _ msg_c) //. }
+          { rewrite map_lookup_imap encσCLook /= /drop_above_bump decide_True //.
+            rewrite /lookup_zero.
+            by simplify_map_eq. }
+          iSplitL "F"; first rewrite decide_True.
+          * iExists P_full'.
+            simpl.
+            rewrite bumperSome.
+            iFrame "PFullEquiv'".
+            iApply (monPred_mono with "F").
+            solve_view_le.
+          * split; first done.
+            rewrite lookup_fmap fmap_None /drop_above.
+            apply map_filter_lookup_None_2.
+            right.
+            lia.
+          * iApply (big_sepM2_impl with "predFRRest").
+            iIntros "!>" (t msg_r encσ_r [? msgRLook]%lookup_delete_Some [_ encσRLook]%lookup_delete_Some) "predR".
+            iSpecialize ("predR" with "[$]").
+            assert (t ≤ t_c).
+            { apply lookup_fmap_Some in msgRLook as (? & _ & msgRLook).
+              by apply map_filter_lookup_Some_1_2 in msgRLook. }
+            rewrite decide_False; last (rewrite not_and_l; left; lia).
+            iApply (encoded_predicate_holds_mono with "predR").
+            solve_view_le.
+        + iExists encp_pers, t_c, t_c, encσ_c', (discard_msg_views msg_c).
+          iSplitPure; first rewrite restrict_lookup_elem_of //.
+          iSplitPure.
+          { subst offsets'.
+            rewrite lookup_fmap restrict_lookup_elem_of; first rewrite OCVLook' //.
+            rewrite elem_of_dom //. }
+          iSplitPure.
+          { rewrite map_lookup_imap encσCLook /= /drop_above_bump decide_True //.
+            - rewrite /safe_bumper bumperSome //.
+            - rewrite /lookup_zero.
+              by simplify_map_eq. }
+          iSplitPure.
+          { rewrite lookup_fmap (map_filter_lookup_Some_2 _ _ _ msg_c) //. }
+          rewrite assoc.
+          iSplitR.
+          * rewrite /lookup_zero.
+            rewrite ?restrict_lookup_elem_of //.
+            rewrite /view_to_zero lookup_fmap.
+            destruct (global_pview !! ℓ); last done.
+            simpl.
+            iSplitPure; first done.
+            iApply persisted_persisted_loc; last done.
+            by eapply view_to_zero_lookup.
+          * iExists P_pers'.
+            iFrame "∗#". }
+
+    (* invoke base logic nextgen begins *)
+    iDestruct (heap_ctx_next_generation _ _ _ Hcrash with "heap") as ">(% & OCV' & #mainpicked & heap)".
+    iDestruct (crashed_at_offset_agree with "crashed_at_offset OCV'") as %<-.
+    iClear "OCV'".
+    iPoseProof (offset_auth_picked_out with "mainpicked offsets") as "offsets".
+    (* invoke base logic nextgen ends *)
+
+    (* [ |==> ] *)
     iModIntro.
+    (* [ ▷ ] *)
+    iModIntro.
+    (* [ ⚡==> ] *)
+    iModIntro.
+    iDestruct "crashed_at_offset" as (? ?) "[picked_in OVOCV]".
+    iPickedInAgree "mainpicked picked_in".
+    iDestruct "allBumpers" as "[last_all_bumpers allBumpers]".
+    iDestruct "allOrders" as "[last_all_orders allOrders]".
+    iDestruct "history" as "[last_history history]".
+    iDestruct "historyFragmentsNG" as "[#lastHistoryFragments historyFragmentsNG]".
+    
+    iMod (lastgen_ghost_map_auth_persist with "last_all_bumpers") as "#last_all_bumpers".
+    iMod (lastgen_ghost_map_auth_persist with "last_all_orders") as "#last_all_orders".
+    iMod (lastgen_full_map_persist with "last_history") as "#last_history".
 
-    iDestruct "crashed_at_offset" as (OV' t) "[picked crashed]".
-    iPickedInAgree "mainpicked picked".
-    iAssert (crashed_at_offset (OCV `view_add` CV))%I as "#crashed_at_offset".
-    { by iExists _. }
-    iSpecialize ("ptsMap" with "crashed_at_offset").
-    iSpecialize ("history" with "crashed_at_offset").
-    iDestruct ("historyFragmentsNG" with "crashed_at_offset") as "historyFragments".
-    iSpecialize ("atLocsHistories" with "crashed_at_offset").
-    iDestruct "full_predicates" as (OCV') "[full_predicates picked]".
-    iAssert ⌜ OCV' = OCV `view_add` CV ⌝%I as %->.
-    { iDestruct (gen_picked_in_agree with "mainpicked picked") as %eq.
-      by simplify_eq. }
-    iClear "picked".
-    iSpecialize ("physHists" with "crashed_at_offset").
-    iDestruct "read_predicates" as (OCV') "[read_predicates picked]".
-    iAssert ⌜ OCV' = OCV `view_add` CV ⌝%I as %->.
-    { iDestruct (gen_picked_in_agree with "mainpicked picked") as %eq.
-      by simplify_eq. }
-    iClear "picked".
-    iDestruct "pers_predicates" as (OCV') "[pers_predicates picked]".
-    iAssert ⌜ OCV' = OCV `view_add` CV ⌝%I as %->.
-    { iDestruct (gen_picked_in_agree with "mainpicked picked") as %eq.
-      by simplify_eq. }
-    iClear "picked".
-    iSpecialize ("allOrders" with "crashed_at_offset").
-    iDestruct "naLocs" as (OCV') "[naLocs picked]".
-    iAssert ⌜ OCV' = OCV `view_add` CV ⌝%I as %->.
-    { iDestruct (gen_picked_in_agree with "mainpicked picked") as %eq.
-      by simplify_eq. }
-    iClear "picked".
-    iDestruct "atLocs" as (OCV') "[atLocs picked]".
-    iAssert ⌜ OCV' = OCV `view_add` CV ⌝%I as %->.
-    { iDestruct (gen_picked_in_agree with "mainpicked picked") as %eq.
-      by simplify_eq. }
-    iClear "picked".
-    iSpecialize ("naView" with "crashed_at_offset").
-    iSpecialize ("allBumpers" with "crashed_at_offset").
+    (* multiple places need [frag_history_at_crash] *)
+    iAssert (frag_history_at_crash)%I as "#frag_impl".
+    { iIntros (??????????).
+      iDestruct ("historyFragmentsNG" with "[OVOCV]") as "#historyFragmentsNG".
+      { by iExists _. }
+      iModIntro.
+      iIntros "OVOCV' %OCVLook' knowOrder knowBumper fragHist %".
+      iDestruct (crashed_at_both_agree with "OVOCV OVOCV'") as %[ <- <- ].
+      (* lookup bumper *)
+      iDestruct "knowBumper" as "[% knowBumper]".
+      iDestruct (lastgen_ghost_map_lookup with "last_all_bumpers knowBumper") as %?.
+      (* lookup (encoded) state *)
+      pose (tC := OCV' !!0 ℓ).
+      assert (ℓ ∈ dom bumpers) by (apply elem_of_dom; by eexists).
+        assert (ℓ ∈ dom phys_hists) as [phys_hist ?]%elem_of_dom by set_solver.
+      assert (ℓ ∈ dom abs_hists) as [abs_hist ?]%elem_of_dom by set_solver.
+      assert (∃ eσ_c, abs_hist !! tC = Some eσ_c)
+        as (eσ_c & ?).
+      { destruct Hcrash as [store PV pIncl cut]. simpl in *.
+        assert (is_Some (CV !! ℓ)) as [[t_c'] tCLook'].
+        { rewrite elem_of_dom lookup_merge in OCVLook'.
+          destruct (OCV !! ℓ) eqn:Heqn; rewrite Heqn /= in OCVLook'.
+          + rewrite -elem_of_dom.
+            pose proof (elem_of_subseteq (dom PV) (dom CV)) as [Hsubset _].
+            specialize (Hsubset ltac:(apply view_le_dom_subseteq; done)).
+            apply Hsubset.
+            pose proof (elem_of_subseteq (dom OCV) (dom PV)) as [Hsubset' _].
+            apply Hsubset'; first done.
+            rewrite elem_of_dom. by eexists.
+          + destruct (CV !! ℓ); done. }
+        (* for the timestamp, we need to go through physical history first *)
+        assert (tC ∈ dom phys_hist) as physHistLook.
+        { simpl in physHistsEq.
+          apply consistent_cut_valid_slice in cut as valid.
+          apply (valid_slice_lookup _ ℓ t_c' _ (drop_prefix phys_hist (OCV !!0 ℓ))) in valid; [ | done | ].
+          - rewrite drop_prefix_lookup in valid.
+            subst tC.
+            rewrite view_add_lookup_zero {2}/lookup_zero tCLook' /=.
+            rewrite elem_of_dom comm //.
+          - symmetry.
+            eapply (map_Forall_lookup_1 _ _ _ _ physHistsEq); done. }
+        apply (map_Forall_lookup_1 _ _ ℓ (phys_hist, abs_hist)) in domAbsHistPhysHist;
+          last rewrite map_lookup_zip_Some //.
+        rewrite domAbsHistPhysHist in physHistLook.
+        by apply elem_of_dom. }
+      iDestruct (big_sepM_lookup _ _ ℓ with "historyFragmentsNG") as "ℓhistory".
+      { rewrite /abs_hist_trans restrict_lookup_elem_of // map_lookup_imap /per_loc_trans.
+        simplify_map_eq.
+        done. }
+      iDestruct (big_sepM_lookup _ _ tC with "ℓhistory") as "knowFragC".
+      { rewrite /drop_bump_map map_lookup_imap.
+        simplify_map_eq.
+        rewrite /drop_above_bump decide_True //. }
+      assert (OCV !!0 ℓ ≤ OCV' !!0 ℓ).
+      { rewrite view_add_lookup_zero.
+        lia. }
+      iSplit; first done.
+      assert (t ≤ OCV' !!0 ℓ) by (subst OCV'; lia).
+      (* lookup [bumperSome] *)
+      iDestruct (big_sepM2_lookup _ _ _ ℓ with "bumperSome") as %bumperSome.
+      { done. } { done. }
+      apply (map_Forall_lookup_1 _ _ tC eσ_c) in bumperSome as [eσ_c' bumperSome]; last done.
+      (* lookup order *)
+      iDestruct (lastgen_ghost_map_lookup with "last_all_orders knowOrder") as %?.
+      iDestruct (big_sepM2_lookup _ _ _ ℓ with "ordered") as %ordered.
+      { done. } { done. }
+      (* lookup [σ] *)
+      iDestruct "fragHist" as (eσ ?) "last_entry".
+      iDestruct (lastgen_full_map_frag_entry with "[$] [$]") as %(? & ? & ?).
+      simplify_map_eq.
+      assert (∃ σ_c, decode eσ_c = Some σ_c ∧ σ ⊑ σ_c) as (σ_c & ? & ?).
+      { destruct (decide (t = tC)) as [-> | ].
+        + exists σ. by simplify_map_eq.
+        + specialize (ordered t tC eσ eσ_c ltac:(lia) ltac:(done) ltac:(done)).
+          apply encode_relation.encode_relation_inv in ordered as (σ' & σ_c & ? & ? & ?).
+          exists σ_c.
+          by simplify_map_eq. }
+      iExists σ_c.
+      iSplit; first done.
+      iSplit.
+      + iExists eσ_c, _.
+        iSplit; first by iExists _.
+        iSplit; first done.
+        iDestruct (big_sepM_lookup _ _ ℓ with "lastHistoryFragments") as "lastHist".
+        { done. }
+        iDestruct (big_sepM_lookup _ _ tC with "lastHist") as "crashFrag".
+        { done. }
+        done.
+      + iExists eσ_c'.
+        apply encode_bumper_Some_decode in bumperSome as (σ_c' & ? & ?).
+        simplify_map_eq.
+        rewrite decode_encode.
+        iSplit; first done.
+        done. }
+
+    iMod "heap" as "[#persisted heap]".
+    
+    iSpecialize ("predsHold" with "[]").
+    { iFrame "frag_impl persisted".
+      iExists OCV, OCV'.
+      iDestruct "crashedRely" as (OPV) "[rely _]".
+      iExists OPV.
+      iFrame "rely OVOCV".
+      iPureIntro.
+      subst OCV'.
+      rewrite map_eq_iff.
+      intros ℓ.
+      rewrite view_sub_lookup /lookup_zero /view_add lookup_merge.
+      destruct (OCV !! ℓ) as [[] | ] eqn:Heq1; destruct (CV !! ℓ) as [[] | ] eqn:Heq2;
+        rewrite ?Heq1 ?Heq2 /= //; try (do 2 f_equiv; lia).
+      (* this is impossible because [dom OCV ⊆ dom PV ⊆ dom CV]. *)
+      destruct Hcrash as [store PV pIncl cut]. simpl in *.
+      assert (ℓ ∈ dom CV) as [? ?]%elem_of_dom; last congruence.
+      apply (elem_of_weaken _ (dom PV)); last by apply dom_included.
+      apply (elem_of_weaken _ (dom OCV)); last done.
+      rewrite elem_of_dom //. }
     iDestruct (big_sepM2_sep with "predsHold") as "[predsFullReadHold predsPersHold]".
+    (* [ |==> ] *)
     iModIntro.
-    iExistsN.
-    iFrame "ptsMap physHists history historyFragments full_predicates read_predicates pers_predicates allOrders naLocs atLocs naView allBumpers offsets".
-    iFrame "predsFullReadHold predsPersHold".
+
+    iAssert (crashed_at_offset OCV')%I as "OCV'".
+    { by iExists _. }
+
+    iDestruct "naView" as "[_ naView]".
+    
+    Ltac solve_crashed_at hyps :=
+      match hyps with
+      | nil => idtac
+      | cons ?H ?hyps' => 
+          (* Try to apply your tactic to the head of the list *)
+          (iSpecialize (H with "OCV'")); 
+          solve_crashed_at hyps'
+      end.
+    
+    solve_crashed_at ["ptsMap"; "physHists"; "full_predicates"; "read_predicates"; "pers_predicates"; "naView";
+                      "allOrders"; "naLocs"; "atLocs"; "history"; "historyFragmentsNG"; "allBumpers"; "atLocsHistories"].
+
+    iFrame "frag_impl heap".
+    iExists (drop_above_map OCV' phys_hists), (abs_hist_trans bumpers OCV' abs_hists), (restrict (dom OCV') $ view_to_zero global_pview),
+            (restrict (dom OCV') predicates_full), (restrict (dom OCV') predicates_read), (restrict (dom OCV') predicates_pers),
+            (restrict (dom OCV') orders), (restrict (dom OCV') bumpers).
+    iExists (na_locs ∩ dom OCV'), (at_locs ∩ dom OCV'), offsets', (const ∅ <$> restrict (dom OCV') na_views).
+
+    iFrame "ptsMap physHists full_predicates read_predicates pers_predicates naView offsets
+            allOrders naLocs atLocs history historyFragmentsNG allBumpers predsPersHold".
     iSplit. (* [#crashedRely] *)
     { iDestruct "crashedRely" as (?) "[rely ?]". iExists _. iApply "rely". }
-    iSplitPure.
-    { rewrite dom_fmap_L restrict_dom_L -offsetsDom.
-      apply dom_imap_L.
-      intros ℓ; split; intros H.
-      - apply elem_of_intersection in H.
-        rewrite /drop_above_hist.
-        destruct H as [[hist ?]%elem_of_dom [[t] ->]%elem_of_dom].
-        exists hist. split; first done.
-        by simpl.
-      - destruct H as (hist & Hdom%elem_of_dom_2 & Hdrop%fmap_is_Some%elem_of_dom).
+    iSplit. (* oldViewsDiscarded *)
+    { iApply (big_sepM2_impl_dom_subseteq with "oldViewsDiscarded").
+      { rewrite /drop_above_map.
+        etrans; first apply dom_imap_subseteq.
+        done. }
+      { subst offsets'.
+        rewrite dom_drop_above_map dom_fmap_L restrict_dom_L.
         set_solver. }
+      iIntros "!>" (ℓ phys_hist offset phys_hist' offset' pLook oLook pLook' oLook' discarded t msg ? msgLook).
+      iPureIntro.
+      assert (ℓ ∈ dom offsets) by by apply elem_of_dom.
+      assert (discard_msg_views <$> drop_above offset' phys_hist = phys_hist') as <-.
+      { rewrite /drop_above_map map_lookup_imap pLook /= in pLook'.
+        rewrite /drop_above_hist in pLook'.
+        subst offsets'.
+        apply lookup_fmap_Some in oLook' as ([] & <- & oLook').
+        rewrite restrict_lookup_elem_of // in oLook'.
+        rewrite oLook' /= in pLook'.
+        by simplify_eq. }
+      apply lookup_fmap_Some in msgLook as (? & <- & ?).
+      rewrite /discard_msg_views /= //. }
+    (* iSplitPure. *)
+    (* { rewrite dom_fmap_L restrict_dom_L -offsetsDom. *)
+    (*   apply dom_imap_L. *)
+    (*   intros ℓ; split; intros H. *)
+    (*   - apply elem_of_intersection in H. *)
+    (*     rewrite /drop_above_hist. *)
+    (*     destruct H as [[hist ?]%elem_of_dom [[t] ->]%elem_of_dom]. *)
+    (*     exists hist. split; first done. *)
+    (*     by simpl. *)
+    (*   - destruct H as (hist & Hdom%elem_of_dom_2 & Hdrop%fmap_is_Some%elem_of_dom). *)
+    (*     set_solver. } *)
+    (* locsDisjoint *)
     iSplitPure; first set_solver.
-    iSplitPure.
+    iSplitPure. (* histDomLocs *)
     { rewrite dom_abs_hist_trans; set_solver. }
-    iSplitPure; first (rewrite restrict_dom_L; set_solver).
-    iSplitPure; first admit. (* [shared_locs_inv] *)
+    (* naViewsDom *)
+    iSplitPure; first (rewrite dom_fmap_L restrict_dom_L; set_solver).
+    (* [shared_locs_inv] *)
+    iSplitPure.
+    { rewrite /shared_locs_inv.
+      rewrite /map_map_Forall.
+      eapply map_Forall_subseteq. { apply restrict_subseteq. }
+      intros ℓ hist look t newMsg histLook.
+      apply map_lookup_zip_with_Some in look as (hist' & off & -> & look & offsetsLook).
+      rewrite map_lookup_imap in look.
+      apply bind_Some in look as (hist & ? & look).
+      assert (discard_msg_views <$> drop_above off hist = hist') as <-.
+      { rewrite /drop_above_hist -lookup_fmap in look.
+        apply lookup_fmap_Some in look as ([] & <- & look).
+        f_equiv.
+        f_equiv.
+        subst offsets' OCV'.
+        simplify_map_eq.
+        rewrite -lookup_fmap in offsetsLook.
+        apply lookup_fmap_Some in offsetsLook as (? & <- & offsetsLook).
+        apply restrict_lookup_Some in offsetsLook as [offsetsLook _].
+        by simplify_map_eq. }
+      rewrite drop_prefix_fmap in histLook.
+      apply lookup_fmap_Some in histLook as ([] & <- & histLook). 
+      apply drop_prefix_drop_above in histLook as [? ?].
+      split; last done.
+      rewrite /discard_msg_views /= view_lookup_zero_empty //. }
     iSplitL "atLocsHistories".
     { rewrite -restrict_abs_hist_trans.
       iDestruct (big_sepM_impl_dom_subseteq _ _ _
-                   (restrict (at_locs ∩ dom (OCV `view_add` CV))
-                      (abs_hist_trans bumpers (OCV `view_add` CV) abs_hists))
+                   (restrict (at_locs ∩ dom OCV')
+                      (abs_hist_trans bumpers OCV' abs_hists))
                   with "atLocsHistories []") as "[$ _]".
       - rewrite ?restrict_dom_L. set_solver.
       - iIntros "!>" (ℓ abs_hist abs_hist' absHistsLook absHistsLook') "full_entry".
         assert (abs_hist = abs_hist') as ->; last done.
-        destruct (decide (ℓ ∈ dom (OCV `view_add` CV)));
+        destruct (decide (ℓ ∈ dom OCV'));
           last (rewrite restrict_lookup_not_elem_of // in absHistsLook'; set_solver).
         destruct (decide (ℓ ∈ at_locs));
           last (rewrite restrict_lookup_not_elem_of // in absHistsLook'; set_solver).
@@ -441,12 +786,15 @@ Section wpr.
         rewrite ?restrict_lookup_elem_of //; last set_solver.
         congruence. }
     iSplit; first admit. (* [ordered] *)
-    iSplit; first admit. (* [histPViewDoms] *)
-
-    (* TODO: hard parts *)
-    (*  * [predicatesHold]: *)
-  Admitted.
-  
+    (* [histPViewDoms] *)
+    iSplitPure.
+    { rewrite dom_abs_hist_trans; last set_solver.
+      rewrite restrict_dom_L /view_to_zero dom_fmap_L.
+      set_solver. }
+    iSplitL "predsFullReadHold"; first rewrite map_imap_drop_OCV_clear_restrict //.
+    
+    
+    
   Lemma idempotence_wpr
       s E1 e e_rec Φ Φr Φc:
     ⊢ validV (store_view e.(ts_view)) -∗
@@ -457,7 +805,7 @@ Section wpr.
   Proof.
     iIntros "#validV Hwpc #Hidemp".
     iApply (idempotence_wpr
-              (λ OCV, crashed_at_offset OCV ∗ crashed_in_impl OCV)%I
+              (frag_history_at_crash)
               extra_state_nextgen
               s E1 e (e_rec `at` ⊥) _ _ _ (Φc ⊥)
                             with "[Hwpc] [Hidemp]").
@@ -475,10 +823,11 @@ Section wpr.
     iApply (plainly_mono with "[$]").
     iIntros "Hidemp Φc".
     iSpecialize ("Hidemp" with "Φc").
-    iModIntro.
     rewrite /nextgen.nextgen /=.
-    iIntros "!> %OCV [? ?] validV".
-    iDestruct ("Hidemp" $! OCV with "[$] [$]") as "Hwpc".
+    iIntros "!> !> Hfrag".
+    iSpecialize ("Hidemp" with "Hfrag").
+    iIntros "validV".
+    iDestruct "Hidemp" as "Hwpc".
     (* rewrite monPred_at_and monPred_at_embed. *)
     iSplit; first done.
     rewrite wpc_eq /wpc_def /wpc /=.
