src/high/weakestpre/at/faa.v
@@ -11,7 +11,7 @@ From self.base Require Import generational_resources primitive_laws.
 From self.high Require Import wrappers monpred_simpl protocol locations crash_weakestpre weakestpre.
 From self.high.modalities Require Import post_fence_sync_advanced.
 From self.high.lib Require Import abstract_state increasing_map.
-From self.high.weakestpre.at Require Import prelude cas.
+From self.high.weakestpre.at Require Import prelude.
 
 From self Require Export lang.
 From self.high Require Export dprop.
@@ -87,7 +87,7 @@ Section wp_at.
     rewrite ?monPred_at_big_sepM.
     iDestruct (big_sepM_lookup with "absHist") as "hist"; first done.
     iEval (rewrite monPred_at_embed) in "hist".
-    iDestruct (history_full_entry_frag_lookup with "fullHist hist")
+    iDestruct (know_full_encoded_history_lookup with "fullHist hist")
       as %(encσ_i & Hlookσ_i & Hdecodeσ_i).
 
     iApply (wp_faa_alt with "[#] [$offsets $pts $val]").
@@ -278,7 +278,7 @@ Section wp_at.
     iMod (auth_map_map_lookup _ _ _ _ t_l with "physHists") as "[physHists #know_msg_l]".
     { done. } { done. }
     iAssert (know_frag_history_loc ℓ t_l σ_l)%I as "#know_σ_l".
-    { rewrite /know_frag_history_loc /frag_entry_unenc.
+    { rewrite /know_frag_history_loc.
       iExists encσ_l.
       iPoseProof (big_sepM_lookup _ _ t_l with "frags") as "$"; done. }
     
@@ -340,7 +340,6 @@ Section wp_at.
         lia. }
       { destruct TV as [[? ?] ?].
         iDestruct (into_no_buffer_at with "predF") as "predF".
-        { apply full_nobuf. }
         destruct (decide _).
         - iApply (predicate_holds_phi with "predFullEquiv"); first reflexivity.
           iApply (monPred_mono with "predF").
@@ -414,7 +413,6 @@ Section wp_at.
     2: {
       eapply map_dom_eq_lookup_None; first done.
       apply nolater. lia. }
-    rewrite -know_protocol_unfold.
     iFrameF "locationProtocol".
     iSplitPure.
     { apply: increasing_map_insert_last; try done. lia.
@@ -442,6 +440,5 @@ Section wp_at.
     etrans; first apply incl.
     etrans; first apply incl2.
     repeat split; solve_view_le.
-    Unshelve. all: done.
   Qed.
 End wp_at.
